Start on different variable types. Also restructure.

Examples/SimpleIter.lean
@@ -1,7 +1,6 @@
 -- import LeanBoogie.BoogieDsl
 import LeanBoogie.ITree
-import LeanBoogie.Boogie
-import LeanBoogie.Mem
+import LeanBoogie.State
 import Auto
 import Aesop
 
@@ -13,42 +12,50 @@ set_option trace.auto.smt.result true
 set_option trace.auto.printLemmas true
 set_option auto.smt.trust true
 set_option auto.smt.solver.name "z3"
-set_option pp.fieldNotation.generalized false
+-- set_option pp.fieldNotation.generalized false
 
 -- Very simple example which can be proven using unrolling or a congruence on the while loop
 
-def p1 : ITree MemEv Unit := do
-  Mem.write "i" 0
-  while_ (Mem.read "i" >>= (fun i => return i < 3)) do
-    Mem.update "i" (. + 1)
-    Mem.update "x" (. + 2)
-  Mem.write "i" 0 -- need to set `i` to 0 afterwards, otherwise the programs compute the same `x` but not `i`.
+def Γ : Con := [.int, .int]
+def i : Var Γ .int := .vz
+def x : Var Γ .int := .vs .vz
 
-def p2 : ITree MemEv Unit := do
-  Mem.write "i" 0
-  while_ (return (<- Mem.read "i") < 6) do
-    Mem.update "x" (. + 1)
-    Mem.update "i" (. + 1)
-  Mem.write "i" 0
+def p1 : ITree (Mem Γ) Unit := do
+  Mem.write i 0
+  While (Mem.read i >>= (fun i => return i < 3)) do
+    Mem.update i (. + 1)
+    Mem.update x (. + 2)
+  Mem.write i 0 -- need to set `i` to 0 afterwards, otherwise the programs compute the same `x` but not `i`.
 
-example : (interp p1) = (interp p2)  := by
+def p2 : ITree (Mem Γ) Unit := do
+  Mem.write i 0
+  While (return (<- Mem.read i) < 6) do
+    Mem.update x (. + 1)
+    Mem.update i (. + 1)
+  Mem.write i 0
+
+set_option trace.split.failure true
+
+-- set_option maxHeartbeats 99999999
+example : interp p1 = interp p2 := by
   rw [p1, p2]
   -- 1. unroll loops
   conv =>
     lhs
-    rw [while_unroll1']
-    rw [while_unroll1']
-    rw [while_unroll1']
-    rw [while_unroll1']
-    rw [while_unroll1']
-  conv => rhs; rw [while_unroll1', while_unroll1', while_unroll1', while_unroll1', while_unroll1', while_unroll1', while_unroll1', while_unroll1']
-  simp [ITree.ite]
+    rw [while_fp]
+    rw [while_fp]
+    rw [while_fp]
+    rw [while_fp]
+    rw [while_fp]
+  conv => rhs; rw [while_fp, while_fp, while_fp, while_fp, while_fp, while_fp, while_fp, while_fp]
 
   -- 2. Push `interp` inwards as far as possible,
   -- this will change `ITree.{pure, bind, iter, ite, read, write}`
   -- into `Boog.{pure, bind, iter, ite, read, write}`
-  simp [interp_bind, interp_write, interp_ite, interp_pure,
-    Mem.update, interp_write, interp_read, skip, ITree.ite]
+  simp [interp_pure, interp_bind, interp_write, interp_read, interp_ite,
+    Mem.update]
+  rw [interp_read] -- for some reason the `simp` above doesn't do this?
+  rw [interp_read]
   -- Our goal is now of form `b1 b2 : (S -> ITree ∅ (A × S)) ⊢ ∀σ:S, (b1 σ) (b2 σ)`, with the predominant `bind` being `Boog.bind`.
 
   -- 3. Push state `σ` inwards as far as possible. This allows us to apply `pure_bind` and obtain
@@ -57,19 +64,80 @@ example : (interp p1) = (interp p2)  := by
   -- However, we know that `ITree.bind (Boog.read v σ) k` is actually `ITree.bind (ITree.pure (σ v, σ)) k`, which simplifies to `k (σ v) σ` via `pure_bind`. Similar for `.write`.
   ext σ
   unfold StateT.run
-  simp only [Boogie.bind_push_state, Boogie.ite_push_state]
-  simp only [Boogie.read, Boogie.write, BoogieState.update.eq_unfold]
-  simp only [pure_bind, Nat.ofNat_pos, dite_eq_ite, ↓reduceDIte, ↓reduceIte, String.reduceEq, zero_add, Nat.one_lt_ofNat, Int.reduceAdd, Int.reduceLT, lt_self_iff_false]
-  simp_all only [↓reduceIte]
+  simp only [State.bind_push_state, State.ite_push_state]
+  simp only [State.read, State.write]
 
+  /- Note how this `simp only [pure_bind]` transforms
+    ```
+    let res ← Pure.pure (PUnit.unit, ConA.set σ i 0)
+    let res ← Pure.pure (ConA.get res.2 i, res.2)
+    let res ← if res.1 < 3 then ...
+    ```
+    into
+    ```
+    let res ← if ConA.get (ConA.set σ i 0) i < 3 then ...
+    ```
+    and then we use `ConA.update_lww` (last write wins) to obtain
+    ```
+    let res ← if 0 < 3 then ...
+    ```
+  -/
+  have i_ne_x : i ≠ x := sorry
+  simp [↓pure_bind, Nat.ofNat_pos, ↓reduceIte, zero_add,
+    Nat.one_lt_ofNat, Int.reduceAdd, Int.reduceLT, lt_self_iff_false,
+    ConA.update_get, ConA.update_lww,
+    ConA.get_irrelevant_set_Var i x i_ne_x, -- ! Will need to add every permutation of this... ?
+    ConA.get_irrelevant_set_Var x i (by aesop),
+  ]
   dsimp [Pure.pure, ITree.pure]
+  congr 2
+  /- Now we have an equality on `ConA Γ`
+    On the left side of the equality we have the following, which we still need to simplify:
+    ```
+    σ
+    |>.set i 1
+    |>.set x (σ.get x + 2)
+    |>.set i 2
+    |>.set x (σ.get x + 2 + 2)
+    |>.set i 3
+    |>.set x (σ.get x + 2 + 2 + 2)
+    ```
+  -/
+  conv =>
+    lhs
+  rw [ConA.grab (γ := (((((σ.set i 1).set x (σ.get x + 2)).set i 2).set x (σ.get x + 2 + 2)).set i 3).set x (σ.get x + 2 + 2 + 2)) i]
+  simp [ConA.update_get, ConA.update_lww,
+    ConA.get_irrelevant_set_Var i x i_ne_x, -- ! Will need to add every permutation of this... ?
+    ConA.get_irrelevant_set_Var x i (by aesop),
+  ]
+  rw [ConA.grab (γ := ((((((σ.set i 1).set x (σ.get x + 2)).set i 2).set x (σ.get x + 2 + 2)).set i 3).set x (σ.get x + 2 + 2 + 2)).set i 3) x]
+  simp [ConA.update_get, ConA.update_lww,
+    ConA.get_irrelevant_set_Var i x i_ne_x, -- ! Will need to add every permutation of this... ?
+    ConA.get_irrelevant_set_Var x i (by aesop),
+  ]
+  -- have : (((((σ.set i 1).set x (σ.get x + 2)).set i 2).set x (σ.get x + 2 + 2)).set i 3).set x (σ.get x + 2 + 2 + 2) =
+  --     id ((((((σ.set i 1).set x (σ.get x + 2)).set i 2).set x (σ.get x + 2 + 2)).set i 3).set x (σ.get x + 2 + 2 + 2)) := rfl
+  -- rw [this]
+  -- rw [<- spread_id]
+  -- simp only [spread]
+
+
   /-
   ret ((), fun v' => if v' = "i" then 0 else if v' = "x" then σ "x" + 2 + 2 + 2 else σ v') =
   ret ((), fun v' => if v' = "i" then 0 else if v' = "x" then σ "x" + 1 + 1 + 1 + 1 + 1 + 1 else σ v')
   -/
 
   -- Our goal is now of form `σ : S ⊢ .ret (a, f σ) = .ret (b, g σ)`
-  congr 2
-  unfold BoogieState at *
+  -- congr 1
   -- 4. Solve by auto :)
   auto
+
+/-
+  σ
+  |>.set i 1
+  |>.set x (σ.get x + 2)
+  |>.set i 2
+  |>.set x (σ.get x + 2 + 2)
+  |>.set i 3
+  |>.set x (σ.get x + 2 + 2 + 2)
+-/
