LeanBoogie/ITree/Monad.lean
@@ -8,20 +8,17 @@ namespace ITree
 
 def pure (a : A) : ITree E A := .ret a
 
-def bind (ta : ITree E A) (tb : A -> ITree E B) : ITree E B := sorry -- TODO: fix
-  -- ITree.corec (β := Sum (ITree E A) (ITree E B)) (fun x =>
-  --   match x with
-  --   | .inl ta =>
-  --     match ta.dest with
-  --     | .ret (.up a : ULift A) =>
-  --       let tb : ITree E B := tb a
-  --       let ret : ITree.Base E B (ITree E B) := tb.dest
-  --       let ret : ITree.Base E B (ITree E A ⊕ ITree E B) := MvFunctor.map (F := TypeFun.ofCurried (n := _) Base) Base.Inr ret
-  --       ret
-  --     | .tau t => .tau (.inl t)
-  --     | .vis e k => .vis e (fun x => .inl (k x))
-  --   | .inr b => Base.replay b Sum.inr
-  -- ) (Sum.inl ta)
+
+def bind (ta : ITree E A) (tb : A -> ITree E B) : ITree E B :=
+  ITree.corec (β := Sum (ITree E A) (ITree E B)) (fun x =>
+    match x with
+    | .inl ta =>
+      match ta.dest with
+      | .ret (.up a : ULift A) => Base.map Sum.inr (tb a).dest
+      | .tau t => .tau (.inl t)
+      | .vis ⟨Ans, e, k⟩ => .vis ⟨Ans, e, (fun x => .inl (k x))⟩
+    | .inr tb => Base.replay tb Sum.inr
+  ) (Sum.inl ta)
 
 instance : Monad (ITree E) where
   pure := pure
