Examples/NonDeterminism/LongestString.lean
@@ -1,0 +1,14 @@
+
+-- Example of nondeterminism:
+-- correct:      `longest("foo", "bar") = "foo"`
+-- also correct: `longest("foo", "bar") = "bar"`
+
+procedure longest(s1: string, s2: string) returns string {
+  goto A, B;
+A:
+  assume |s1| <= |s2|
+  return s2;
+B:
+  assume |s1| >= |s2|
+  return s1;
+}
