Examples/RunFinite.lean
@@ -1,0 +1,29 @@
+import LeanBoogie.ITree
+import LeanBoogie.Mem
+import LeanBoogie.State
+import Aesop
+
+open LeanBoogie ITree
+
+def Γ : Con := [.int, .int]
+def i : Var Γ .int := .vz
+def x : Var Γ .int := .vs .vz
+
+def prog : ITree (Mem Γ) Unit := do
+  while_ (Mem.read i >>= (fun i => return i < 3)) do
+    Mem.update i (. + 1)
+    Mem.update x (. + 2)
+
+def runProg (fuel : Nat) : IO Int := StateT.run' (do
+    let _ <- run prog fuel handle
+    State.read x
+  )
+  default
+
+-- feel free to uncomment the rest
+#eval timeit "" (runProg 3) -- 12ms, x=0
+-- #eval timeit "" (runProg 4) -- 22ms, x=0
+-- #eval timeit "" (runProg 5) -- 50ms, x=2
+-- #eval timeit "" (runProg 10) -- 1.4s, x=2
+-- #eval timeit "" (runProg 15) -- 2.6s, x=4
+-- #eval timeit "" (runProg 20) -- 5.5s, x=6
