LeanBoogie/Effect/Mem.lean
@@ -1,0 +1,52 @@
+import LeanBoogie.ITree
+import LeanBoogie.Types
+import Mathlib.Data.Real.Basic
+
+namespace LeanBoogie
+open ITree (HasEff)
+
+/-
+  # Memory (Effects) in Boogie
+
+  Without interpretation yet. For that, look into `State.lean`.
+-/
+
+-- ## `Mem` Effect
+
+inductive Mem (Γ : Con) : Type -> Type where
+| rd : Var Γ A          -> Mem Γ A
+| wr : Var Γ A -> TyA A -> Mem Γ Unit
+
+def Mem.read  (v : Var Γ A)           : ITree (Mem Γ) A    := .vis (.rd v    ) .ret
+def Mem.write (v : Var Γ A) (val : A) : ITree (Mem Γ) Unit := .vis (.wr v val) .ret
+/-- Apply a pure function to a variable. E.g. `Mem.update x (· + 10)`. -/
+abbrev Mem.update (v : Var Γ A) (f : A -> A) : ITree (Mem Γ) Unit := do
+  let val <- read v
+  write v (f val)
+
+def Mem.read'  (v : Var Γ A)           : ITree (E & Mem Γ) A    := .vis (Mem.rd v    ) .ret
+def Mem.write' (v : Var Γ A) (val : A) : ITree (E & Mem Γ) Unit := .vis (Mem.wr v val) .ret
+
+-- the most general form is like this, with `HasEff`:
+def Mem.read''  [HasEff (Mem Γ) E] (v : Var Γ A)           : ITree E A    := .vis (Mem.rd v    ) .ret
+def Mem.write'' [HasEff (Mem Γ) E] (v : Var Γ A) (val : A) : ITree E Unit := .vis (Mem.wr v val) .ret
+
+private def Γ : Con := [.int, .bv 32, .bool ~> .int]
+private def i : Var Γ .int := .v0
+private def b : Var Γ (.bv32) := .v1
+private def f : Var Γ (.bool ~> .int) := .v2
+private example : ITree (Mem Γ) Unit := do
+  let fn : Bool -> Int <- Mem.read f
+  Mem.write b (fn false)
+
+def merge : ITree (Mem Γ & Mem Δ) A -> ITree (Mem (Γ ++ Δ)) A := sorry
+
+
+/-
+  # The Boogie Way
+-/
+
+axiom Ref : Type
+def C.data : Ref -> Int := sorry
+def C.next : Ref -> Ref := sorry
+def alloc : Ref -> Prop := sorry -- which refs are allocated
