LeanBoogie/Iter.lean
@@ -2,14 +2,86 @@ import LeanBoogie.Notation
 
 namespace LeanBoogie
 
-/-- The monad `M` is equipped with `iter`. -/
-class Iter (M : Type u -> Type v) [Monad M] where
-  iter : {A B : Type u} -> (A -> M (A ⊕ B)) -> A -> M B
+def case [Monad M] (ca : A -> M C) (cb : B -> M C) (ab : M (A ⊕ B)) : M C := do
+  match <- ab with
+  | .inl a => ca a
+  | .inr b => cb b
+
+/-
+  # `Iter`ative monads
+  This does not mention `ITree`s, but we can state some properties nonetheles.
+-/
+
+/-- The monad `M` is equipped with `iter`.
+
+  Implementing this typeclass automatically gives you a few other goodies, such as `loop`, `While`.
+ -/
+class Iter (M : Type u -> Type v) extends Monad M where
+  /-- Repeat `f` until it returns `B`. -/
+  iter : {A B : Type u} -> (f : A -> M (A ⊕ B)) -> (a₀ : A) -> M B
+  -- iterLift : ... := ...
+  -- loop : ... := ...
+  -- While : ... := ...
 
 export Iter (iter)
 
--- class LawfulIter (M : Type -> Type) {equiv : {A : Type} -> M A -> M A -> Prop} [Monad M] [Iter M] : Prop where
---   iter_fp : equiv (iter f a) (iter f a)
+def iterLift [Iter M] (body : A -> M (A ⊕ B)) : (A ⊕ B) -> M (A ⊕ B)
+| .inl a => body a
+| .inr b => return .inr b
+
+/-- `iterOn a₀ f = iter f a₀`. -/
+abbrev iterOn [Iter M] {A B : Type u} (a₀ : A) (f : A -> M (A ⊕ B)) :=
+  iter f a₀
+
+/-- A different phrasing of `iter`.
+
+  From the ITree paper:
+  ```
+  Definition loop (body : C + A → itree E (C + B)) : A → itree E B :=
+    fun a ⇒ iter (fun ca ⇒
+      cb <- body ca ;;
+      match cb with
+      | inl c ⇒ Ret (inl (inl c))
+      | inr b ⇒ Ret (inr b)
+      end) (inr a).
+  ```
+-/
+def loop [Iter M] (body : C ⊕ A -> M (C ⊕ B)) (a : A) : M B :=
+  sorry
+
+-- Maybe use this instead of `Bool` in `While`?
+-- structure DProp : Type u where
+--   P : Prop
+--   decide : Decidable P
+
+/-- Combinator for writing `while` loops, expressed in terms of `iter`.
+
+  Uppercase because `while` is a keyword in Lean. -/
+def While [Iter M] (c : M Bool) (body : M Unit) : M Unit :=
+  iter (fun () => do
+    if (<- c) then
+      body
+      return .inl ()
+    else
+      return .inr ()
+  )
+  ()
+
+class LawfulIter (M : Type /- u -/ -> Type v) [Iter M] : Prop where
+  iter_fp' {f : A -> M (A ⊕ B)} {a₀ : A}
+    : iter f a₀
+    = do
+      match <- f a₀ with
+      | .inl a => iter f a
+      | .inr b => return b
+  while_fp {c : M Bool} : While c body = do if (<- c) then body; While c body
+  /-- Unroll `iter` once. Note that the first case is `(fun a => iter f a)` instead of `iter f`,
+    so that we can apply `iter_fp` multiple times. -/
+  iter_fp {f : A -> M (A ⊕ B)} {a₀ : A} : iter f a₀ = case (fun a => iter f a) pure (f a₀) := iter_fp'
+  iter_fp'' {f : A -> M (A ⊕ B)} : iter f = fun a₀ => case (iter f) pure (f a₀) := funext (fun a => iter_fp (a₀ := a))
+
+export LawfulIter (iter_fp iter_fp' iter_fp'' while_fp)
+
 -- /-- We can unroll `iter f`. -/
 -- theorem iter_fp {f : KTree E A (A ⊕ B)} : iter f ~~~ f >>> case (iter f) id := trustITree "page 9"
 -- theorem iter_fp_nonK {f : KTree E A (A ⊕ B)} : iter f p ~~ f p >>= case (iter f) id := by sorry
